Finished disjoint_memory proof

Access.v
@@ -1,4 +1,5 @@
 From Coq Require Import Arith.Arith.
+From Coq Require Import Lia.
 
 From Coq Require Logic.ClassicalFacts.
 
@@ -47,6 +48,9 @@ Proof.
   intros * Hacc ?. induction Hacc; eauto using access.
 Qed.
 
+Definition well_behaved_access m t :=
+  forall ad, access m t ad -> ad < length m.
+
 Local Axiom excluded_middle : ClassicalFacts.excluded_middle.
 
 Lemma access_dec : forall m t ad,
@@ -59,7 +63,7 @@ Ltac inversion_access :=
   match goal with
     | H : access _ TM_Nil       _ |- _ => inversion H; clear H
     | H : access _ (TM_Num _)   _ |- _ => inversion H; clear H
-    | H : access _ (TM_Loc _)   _ |- _ => inversion H; clear H
+    | H : access _ (TM_Loc _)   _ |- _ => inversion H; subst; clear H
     | H : access _ (TM_New _)   _ |- _ => inversion H; subst; clear H
     | H : access _ (TM_Load _)  _ |- _ => inversion H; subst; clear H
     | H : access _ (TM_Asg _ _) _ |- _ => inversion H; subst; clear H
@@ -149,168 +153,424 @@ Proof.
   intros * ? ? ?. inversion_access; eauto.
 Qed.
 
-Module Mem.
-  Lemma add_preserves_access : forall m t ad v,
+(*****************************************************************************)
+(* Compat ********************************************************************)
+(*****************************************************************************)
+
+Module Compat.
+  Definition compat m m' t := forall ad,
     access m t ad ->
-    access (add m v) t ad.
+    getTM m ad = getTM m' ad.
+
+  Lemma refl : forall m t, 
+    compat m m t.
   Proof.
-    intros * Hacc. induction Hacc; eauto using access.
-    eapply access_mem. destruct (lt_eq_lt_dec ad' (length m)) as [[? | ?] | ?]. 
-    - rewrite (get_add_lt TM_Nil); trivial.
-    - subst. rewrite (get_default TM_Nil) in IHHacc; eauto using Nat.le_refl.
-      inversion_access.
-    - rewrite (get_default TM_Nil) in IHHacc; eauto using Nat.lt_le_incl.
-      inversion_access.
+    intros. unfold compat. trivial.
   Qed.
 
-  Lemma set_preserves_access : forall m t ad ad' v,
-    ~ access m v ad ->
-    access (set m ad' v) t ad ->
-    access m t ad.
+  Lemma sym : forall m m' t, 
+    compat m  m' t ->
+    compat m' m  t. 
   Proof.
-    intros * Hnacc Hacc. remember (set m ad' v) as m'.
-    induction Hacc; inversion Heqm'; subst; eauto using access.
-    match goal with 
-      IH : ~ _ -> access _ (getTM (set _ ?ad1 _) ?ad2) ?ad3 |- _ =>
-        destruct (Nat.eq_dec ad1 ad2); subst;
-        try solve [rewrite (get_set_neq TM_Nil) in IH; eauto using access];
-        destruct (Nat.eq_dec ad2 ad3); subst; eauto using access
+    intros * Hcompat ad Hacc. unfold compat in *.
+    induction Hacc; eauto using access;
+    try solve [symmetry; eauto using access].
+    eapply IHHacc. intros ? ?.
+    eapply Hcompat. eapply access_mem.
+    rewrite (Hcompat _ (access_loc _ _)).
+    trivial.
+  Qed.
+
+  Lemma acc : forall m m' t ad,
+    compat m m' t ->
+    access m  t ad ->
+    access m' t ad.
+  Proof.
+    intros * Hcompat Hacc. unfold compat in *.
+    induction Hacc; eauto using access.
+    eapply access_mem.
+    rewrite <- (Hcompat _ (access_loc _ _)).
+    eapply IHHacc. intros ? ?.
+    eapply Hcompat. eauto using access.
+  Qed.
+
+  Lemma acc_not : forall m m' t ad,
+    compat m m' t ->
+    ~ access m  t ad ->
+    ~ access m' t ad.
+  Proof.
+    intros * ? ? ?. eauto using acc, sym.
+  Qed.
+
+  Corollary access_iff : forall m m' t ad,
+    compat m m' t ->
+    access m t ad <-> access m' t ad.
+  Proof.
+    intros * ?. split; eauto using acc, sym.
+  Qed.
+
+  Lemma inaccessible_address_set : forall m m' t ad v,
+    compat m m' t ->
+    ~ access m t ad ->
+    compat m (set m' ad v) t.
+  Proof.
+    intros * Hcompat Hnacc ad Hacc. unfold compat in *.
+    induction Hacc; try solve [inversion_not_access; eauto using access].
+    match goal with H : ~ access _ _ ?ad' |- _ => 
+      destruct (Nat.eq_dec ad ad'); subst
     end.
-    exfalso. rewrite (get_set_eq TM_Nil) in IHHacc; eauto.
-    eapply not_le. intros F. rewrite (get_default TM_Nil) in Hacc.
-    - inversion_access.
-    - rewrite set_preserves_length. trivial.
+    - exfalso. eauto using access.
+    - rewrite (get_set_neq TM_Nil); eauto using access.
   Qed.
 
-  Local Lemma set_preserves_not_access : forall m t ad ad' v,
-    ~ access m t ad ->
-    ~ access m v ad ->
-    ~ access (set m ad' v) t ad.
+  Lemma inaccessible_address_add : forall m m' t v,
+    compat m m' t ->
+    ~ access m t (length m') ->
+    compat m (add m' v) t.
   Proof.
-    assert (ge_iff_le : forall m n, m >= n <-> n <= m). {
-      intros. split; destruct n; eauto.
-    }
-    assert (forall m ad ad' v,
-      access (set m ad' v) (getTM (set m ad' v) ad') ad ->
-      ad' < length m). {
-      intros * H. eapply not_ge. rewrite ge_iff_le. intros ?.
-      rewrite (get_set_invalid TM_Nil) in H; trivial. inversion H.
-    }
-
-    intros * HnaccT HnaccV F.
-    remember (set m ad' v) as m'.
-    induction F; inversion Heqm'; subst; eauto using access.
-    match goal with H : ~ access _ (TM_Loc ?ad) _ |- _ => 
-      destruct (Nat.eq_dec ad' ad) as [? | Hneq]; subst
-    end. 
-    - match goal with H : ~ access _ (TM_Loc ?ad) _ |- _ => 
-        assert (ad < length m); eauto
-      end. 
-      rewrite (get_set_eq TM_Nil) in F;
-      rewrite (get_set_eq TM_Nil) in IHF; eauto.
-    - eapply not_eq_sym in Hneq.
-      rewrite (get_set_neq TM_Nil) in *; eauto using access.
+    intros * Hcompat Hnacc ad Hacc. unfold compat in *.
+    induction Hacc; try solve [inversion_not_access; eauto using access].
+    destruct (Nat.eq_dec ad (length m')); subst.
+    + exfalso. eauto using access.
+    + destruct (not_eq ad (length m')); trivial.
+      * rewrite (get_add_lt TM_Nil); eauto using access.
+      * specialize (Hcompat ad (access_loc m ad)).
+        rewrite (get_default TM_Nil m') in Hcompat; try lia.
+        rewrite (get_add_gt TM_Nil); trivial.
   Qed.
-End Mem.
+End Compat.
 
-Module Step.
-  Lemma load_ad_access: forall m t t' ad v,
-    t --[EF_Load ad v]--> t' ->
-    access m t ad.
+Corollary inaccessible_address_set_1 : forall m t ad ad' v,
+  ~ access m t ad' ->
+  access (set m ad' v) t ad ->
+  access m t ad.
+Proof.
+  intros * ? ?.
+  eauto using Compat.refl,
+              Compat.sym,
+              Compat.inaccessible_address_set,
+              Compat.acc.
+Qed.
+
+Corollary inaccessible_address_set_2  : forall m t ad ad' v,
+  ~ access m t ad' ->
+  ~ access m t ad ->
+  ~ access (set m ad' v) t ad.
+Proof.
+  intros * ? ?.
+  eauto using Compat.refl, Compat.inaccessible_address_set, Compat.acc_not.
+Qed.
+
+Corollary inaccessible_address_add_1 : forall m t ad v,
+  ~ access m t (length m) ->
+  access (add m v) t ad ->
+  access m t ad.
+Proof.
+  intros * ? ?.
+  eauto using Compat.refl,
+              Compat.sym,
+              Compat.inaccessible_address_add,
+              Compat.acc.
+Qed.
+
+Corollary inaccessible_address_add_2 : forall m t ad v,
+  ~ access m t (length m) ->
+  ~ access m t ad ->
+  ~ access (add m v) t ad.
+Proof.
+  intros * ? ?.
+  eauto using Compat.refl, Compat.inaccessible_address_add, Compat.acc_not.
+Qed.
+
+(*****************************************************************************)
+(* WBA ***********************************************************************)
+(*****************************************************************************)
+
+Module WBA.
+  Lemma destruct_new : forall m t,
+    well_behaved_access m (TM_New t) ->
+    well_behaved_access m t.
   Proof.
-    intros * Hstep.
-    remember (EF_Load ad v) as eff.
-    induction Hstep; eauto using access;
-    inversion Heqeff; subst. eauto using access.
+    intros * ? ?; eauto using access.
   Qed.
 
-
-  Lemma store_not_v_access : forall m t t' ad ad' v,
-    ~ access m t ad ->
-    t --[EF_Store ad' v]--> t' ->
-    ~ access m v ad.
+  Lemma destruct_load : forall m t,
+    well_behaved_access m (TM_Load t) ->
+    well_behaved_access m t.
   Proof.
-    intros * Hnacc ?.
-    remember (EF_Store ad' v) as eff.
-    induction_step; inversion Heqeff; subst; eauto using access.
+    intros * ? ?; eauto using access.
   Qed.
 
-  Lemma store_v_access : forall m t t' ad ad' v,
-    access m v ad ->
-    t --[EF_Store ad' v]--> t' ->
-    access m t ad.
+  Lemma destruct_asg : forall m l r,
+    well_behaved_access m (TM_Asg l r) ->
+    well_behaved_access m l /\ well_behaved_access m r.
   Proof.
-    intros * ? ?. remember (EF_Store ad' v) as eff.
-    induction_step; inversion Heqeff; subst; eauto using access.
+    intros * ?. split; intros ?; eauto using access.
   Qed.
 
-  Lemma store_access_backwards : forall m t t' ad ad' v,
-    t --[EF_Store ad' v]--> t' ->
-    access (set m ad' v) t' ad ->
-    access m t ad.
+  Lemma destruct_seq : forall m t1 t2,
+    well_behaved_access m (TM_Seq t1 t2) ->
+    well_behaved_access m t1 /\ well_behaved_access m t2.
   Proof.
-    intros * Hstep Hacc. 
-    remember (EF_Store ad' v) as eff.
+    intros * ?. split; intros ?; eauto using access.
+  Qed.
+
+  Ltac destruct_wba :=
+    match goal with
+      | H : well_behaved_access _ (TM_New _)   |- _ =>
+          eapply destruct_new in H
+      | H : well_behaved_access _ (TM_Load _)  |- _ =>
+          eapply destruct_load in H
+      | H : well_behaved_access _ (TM_Asg _ _) |- _ => 
+          eapply destruct_asg in H as [? ?]
+      | H : well_behaved_access _ (TM_Seq _ _) |- _ => 
+          eapply destruct_seq in H as [? ?]
+    end.
+
+  Local Lemma wba_load : forall m t,
+    well_behaved_access m t ->
+    well_behaved_access m (TM_Load t).
+  Proof.
+    intros * ? ? ?. inversion_access. eauto.
+  Qed.
+
+  Local Lemma wba_asg : forall m l r,
+    well_behaved_access m l ->
+    well_behaved_access m r ->
+    well_behaved_access m (TM_Asg l r).
+  Proof.
+    intros * ? ? ? ?. inversion_access; eauto.
+  Qed.
+
+  Local Lemma wba_seq : forall m t1 t2,
+    well_behaved_access m t1 ->
+    well_behaved_access m t2 ->
+    well_behaved_access m (TM_Seq t1 t2).
+  Proof.
+    intros * ? ? ? ?. inversion_access; eauto.
+  Qed.
+
+  Local Lemma wba_added_value : forall m v,
+    well_behaved_access (add m v) v ->
+    well_behaved_access (add m v) (TM_Loc (length m)).
+  Proof.
+    intros * ? ? Hacc.
+    remember (add m v) as m'.
+    remember (TM_Loc (length m)) as t'.
+    induction Hacc; inversion Heqt'; subst.
+    - rewrite (get_add_eq TM_Nil) in *; eauto using access.
+    - rewrite add_increments_length. lia.
+  Qed.
+
+  Local Lemma wba_stored_value : forall m t t' ad v,
+    well_behaved_access m t ->
+    t --[EF_Store ad v]--> t' ->
+    well_behaved_access m v.
+  Proof.
+    intros. intros ? ?.
+    remember (EF_Store ad v) as eff.
+    induction_step; try inversion Heqeff; subst;
+    destruct_wba; eauto using access. 
+  Qed.
+
+  Lemma mem_add: forall m t v,
+    well_behaved_access m t ->
+    well_behaved_access (add m v) t.
+  Proof.
+    intros * Hwba ? Hacc. remember (add m v) as m'.
+    induction Hacc; subst; try destruct_wba; eauto.
+    - eapply IHHacc. intros ad'' Hacc''.
+      destruct (lt_eq_lt_dec ad' (length m)) as [[? | ?] | ?]; subst.
+      + rewrite (get_add_lt TM_Nil) in *; eauto using access.
+      + specialize (Hwba (length m) (access_loc m (length m))). lia.
+      + rewrite (get_add_gt TM_Nil) in *; eauto. inversion_access.
+    - rewrite add_increments_length. eauto using access, Nat.lt_lt_succ_r.
+  Qed.
+
+  Lemma mem_set: forall m t ad v,
+    well_behaved_access m t ->
+    well_behaved_access m v ->
+    well_behaved_access (set m ad v) t.
+  Proof.
+    intros * ? ? ? Hacc.
+    rewrite set_preserves_length.
+    remember (set m ad v) as m'.
+    induction Hacc; subst; try destruct_wba; eauto using access.
+    eapply IHHacc. destruct (Nat.eq_dec ad ad'); subst.
+    - rewrite (get_set_eq TM_Nil); eauto using access.
+    - rewrite (get_set_neq TM_Nil) in *; eauto.
+      intros ? ?. eauto using access.
+  Qed.
+
+  Local Lemma none_preservation : forall m t t',
+    well_behaved_access m t ->
+    t --[EF_None]--> t' ->
+    well_behaved_access m t'.
+  Proof.
+    intros. remember (EF_None) as eff.
     induction_step; inversion Heqeff; subst;
-    try inversion_access; eauto using access;
-    destruct (access_dec m v ad);
-    eauto using access, store_v_access, Mem.set_preserves_access.
+    destruct_wba; eauto using wba_load, wba_asg, wba_seq. 
   Qed.
 
-  Lemma store_does_not_grant_access1 : forall m t t' ad ad' v,
-    ~ access m t ad ->
-    t --[EF_Store ad' v]--> t' ->
-    ~ access (set m ad' v) t' ad.
+  Local Lemma alloc_preservation : forall m t t' v,
+    well_behaved_access m t ->
+    t --[EF_Alloc (length m) v]--> t' ->
+    well_behaved_access (add m v) t'.
   Proof.
-    intros * Hnacc ?.
-    remember (EF_Store ad' v) as eff.
+    intros. remember (EF_Alloc (length m) v) as eff.
     induction_step; inversion Heqeff; subst;
-    inversion_not_access;
-    eauto using not_access_load,
-                not_access_asg,
-                not_access_seq,
-                Mem.set_preserves_not_access,
-                store_not_v_access.
+    destruct_wba;
+    eauto using wba_load, wba_asg, wba_seq, mem_add, wba_added_value. 
   Qed.
 
-  Lemma store_does_not_grant_access2 : forall m t t' ad ad' v,
-    ~ access m t ad ->
-    t --[EF_Store ad' v]--> t' ->
-    ~ access m t' ad.
+  Local Lemma load_preservation : forall m t t' ad,
+    well_behaved_access m t ->
+    t --[EF_Load ad (get TM_Nil m ad)]--> t' ->
+    well_behaved_access m t'.
   Proof.
-    intros * Hnacc ?.
-    remember (EF_Store ad' v) as eff.
+    intros. remember (EF_Load ad (get TM_Nil m ad)) as eff.
     induction_step; inversion Heqeff; subst;
-    inversion_not_access;
-    eauto using not_access_load,
-                not_access_asg,
-                not_access_seq,
-                Mem.set_preserves_not_access,
-                store_not_v_access.
+    destruct_wba; eauto using wba_load, wba_asg, wba_seq.
+    intros ? ?. eauto using access.
   Qed.
 
-  Module Store.
-    Lemma address_access : forall m t t' ad v,
-      t --[EF_Store ad v]--> t' ->
+  Local Lemma store_preservation : forall m t t' ad v,
+    well_behaved_access m t ->
+    t --[EF_Store ad v]--> t' ->
+    well_behaved_access (set m ad v) t'.
+  Proof.
+    intros.
+    assert (well_behaved_access m v); eauto using wba_stored_value.
+    remember (EF_Store ad v) as eff.
+    induction_step; inversion Heqeff; subst;
+    destruct_wba; eauto using wba_load, wba_asg, wba_seq, mem_set.
+    intros ? ?. inversion_access.
+  Qed.
+
+  Lemma preservation : forall m m' t t' eff,
+    well_behaved_access m t ->
+    m / t ==[eff]==> m' / t' ->
+    well_behaved_access m' t'.
+  Proof.
+    intros * ? ?. inversion_mstep;
+    eauto using none_preservation, 
+      alloc_preservation,
+      load_preservation,
+      store_preservation.
+  Qed.
+End WBA.
+
+(*****************************************************************************)
+(* Mem ***********************************************************************)
+(*****************************************************************************)
+
+Module Mem.
+  Module Add.
+    Lemma preserves_access : forall m t ad v,
+      access m t ad ->
+      access (add m v) t ad.
+    Proof.
+      intros * Hacc. induction Hacc; eauto using access.
+      eapply access_mem.
+      destruct (lt_eq_lt_dec ad' (length m)) as [[? | ?] | ?]. 
+      - rewrite (get_add_lt TM_Nil); trivial.
+      - subst. rewrite (get_default TM_Nil) in IHHacc; try lia.
+        inversion_access.
+      - rewrite (get_default TM_Nil) in IHHacc; try lia.
+        inversion_access.
+    Qed.
+  End Add.
+
+  Module Set_.
+    Lemma preserves_access : forall m t ad ad' v,
+      ~ access m v ad ->
+      access (set m ad' v) t ad ->
       access m t ad.
     Proof.
-      intros * Hstep. remember (EF_Store ad v) as eff.
+      intros * Hnacc Hacc. remember (set m ad' v) as m'.
+      induction Hacc; inversion Heqm'; subst; eauto using access.
+      match goal with 
+        IH : ~ _ -> access _ (getTM (set _ ?ad1 _) ?ad2) ?ad3 |- _ =>
+          destruct (Nat.eq_dec ad1 ad2); subst;
+          try solve [rewrite (get_set_neq TM_Nil) in IH; eauto using access];
+          destruct (Nat.eq_dec ad2 ad3); subst; eauto using access
+      end.
+      exfalso. rewrite (get_set_eq TM_Nil) in IHHacc; eauto.
+      eapply not_le. intros F. rewrite (get_default TM_Nil) in Hacc.
+      - inversion_access.
+      - rewrite set_preserves_length. trivial.
+    Qed.
+
+    Local Lemma preserves_not_access : forall m t ad ad' v,
+      ~ access m t ad ->
+      ~ access m v ad ->
+      ~ access (set m ad' v) t ad.
+    Proof.
+      assert (ge_iff_le : forall m n, m >= n <-> n <= m). {
+        intros. split; destruct n; eauto.
+      }
+      assert (forall m ad ad' v,
+        access (set m ad' v) (getTM (set m ad' v) ad') ad ->
+        ad' < length m). {
+        intros * H. eapply not_ge. rewrite ge_iff_le. intros ?.
+        rewrite (get_set_invalid TM_Nil) in H; trivial. inversion H.
+      }
+      intros * HnaccT HnaccV F.
+      remember (set m ad' v) as m'.
+      induction F; inversion Heqm'; subst; eauto using access.
+      match goal with H : ~ access _ (TM_Loc ?ad) _ |- _ => 
+        destruct (Nat.eq_dec ad' ad) as [? | Hneq]; subst
+      end. 
+      - match goal with H : ~ access _ (TM_Loc ?ad) _ |- _ => 
+          assert (ad < length m); eauto
+        end. 
+        rewrite (get_set_eq TM_Nil) in F;
+        rewrite (get_set_eq TM_Nil) in IHF; eauto.
+      - eapply not_eq_sym in Hneq.
+        rewrite (get_set_neq TM_Nil) in *; eauto using access.
+    Qed.
+  End Set_.
+End Mem.
+
+(*****************************************************************************)
+(* Step **********************************************************************)
+(*****************************************************************************)
+
+Module Step.
+  Module Alloc.
+    Lemma address_access2 : forall m t t' ad v,
+      t --[EF_Alloc ad v]--> t' ->
+      access m t' ad.
+    Proof.
+      intros. remember (EF_Alloc ad v) as eff.
+      induction_step; inversion Heqeff; subst; eauto using access.
+    Qed. 
+  End Alloc.
+
+  Module Store.
+    Lemma value_access : forall m t t' ad ad' v,
+      access m v ad ->
+      t --[EF_Store ad' v]--> t' ->
+      access m t ad.
+    Proof.
+      intros * ? ?. remember (EF_Store ad' v) as eff.
+      induction_step; inversion Heqeff; subst; eauto using access.
+    Qed.
+
+    Lemma value_not_access : forall m t t' ad ad' v,
+      ~ access m t ad ->
+      t --[EF_Store ad' v]--> t' ->
+      ~ access m v ad.
+    Proof.
+      intros. remember (EF_Store ad' v) as eff.
       induction_step; inversion Heqeff; subst; eauto using access.
     Qed.
   End Store.
 End Step.
 
-(*
-
-Inductive effect : Set :=
-  | EF_None
-  | EF_Alloc (ad : addr) (t : tm)
-  | EF_Load  (ad : addr) (t : tm)
-  | EF_Store (ad : addr) (t : tm)
-  | EF_Spawn (t : tm)
-  .
-
-*)
+(*****************************************************************************)
+(* MStep *********************************************************************)
+(*****************************************************************************)
 
 Module MStep.
   Module None.
@@ -336,17 +596,89 @@ Module MStep.
   End None.
 
   Module Alloc.
+    Local Lemma address_access: forall m m' t t' ad v,
+      m / t ==[EF_Alloc ad v]==> m' / t' ->
+      access m' t' ad.
+    Proof.
+      intros * ?. inversion_mstep. eauto using Step.Alloc.address_access2.
+    Qed.
+
+    Lemma grants_access : forall m m' t t' ad v,
+      well_behaved_access m t ->
+      m / t ==[EF_Alloc ad v]==> m' / t' ->
+      ~ access m t ad /\ access m' t' ad.
+    Proof.
+      intros * Hwba ?. split; eauto using address_access.
+      inversion_mstep. intros F. eapply Hwba in F. lia.
+    Qed.
+
+    Lemma inherits_access : forall m m' t t' ad ad' v,
+      well_behaved_access m t ->
+      ad <> ad' ->
+      access m' t' ad ->
+      m / t ==[EF_Alloc ad' v]==> m' / t' ->
+      access m t ad.
+    Proof.
+      intros * Hwba ? ? Hmstep. inversion_mstep.
+      remember (EF_Alloc (length m) v) as eff.
+      induction_step; inversion Heqeff; subst;
+      WBA.destruct_wba; try inversion_access; eauto using access; try lia.
+      - rewrite (get_add_eq TM_Nil) in *.
+        eapply access_new; eapply inaccessible_address_add_1; eauto. intros F.
+        specialize (Hwba (length m) F). lia.
+      - eapply access_asg2; eapply inaccessible_address_add_1; eauto. intros F.
+        match goal with Hwba : well_behaved_access m ?t |- _ =>
+          specialize (Hwba (length m) F); lia
+        end.
+      - eapply access_asg1; eapply inaccessible_address_add_1; eauto. intros F.
+        match goal with Hwba : well_behaved_access m ?t |- _ =>
+          specialize (Hwba (length m) F); lia
+        end.
+      - eapply access_seq2; eapply inaccessible_address_add_1; eauto. intros F.
+        match goal with Hwba : well_behaved_access m ?t |- _ =>
+          specialize (Hwba (length m) F); lia
+        end.
+    Qed.
+
     Lemma preserves_access : forall m m' t t' ad ad' v,
       access m t ad ->
       m / t ==[EF_Alloc ad' v]==> m' / t' ->
       access m' t' ad.
     Proof.
-      intros * ? ?. inversion_mstep.
-      remember (EF_Alloc (length m) v) as eff.
+      intros. inversion_mstep. remember (EF_Alloc (length m) v) as eff.
       induction_step; inversion Heqeff; subst;
-      inversion_access; eauto using access, Mem.add_preserves_access.
+      inversion_access; eauto using access, Mem.Add.preserves_access.
       eapply access_mem. rewrite (get_add_eq TM_Nil).
-      eauto using Mem.add_preserves_access.
+      eauto using Mem.Add.preserves_access.
+    Qed.
+
+    Lemma preserves_not_access : forall m m' t t' ad ad' v,
+      well_behaved_access m t ->
+      ad <> ad' ->
+      ~ access m t ad ->
+      m / t ==[EF_Alloc ad' v]==> m' / t' ->
+      ~ access m' t' ad.
+    Proof.
+      intros * Hwba ? ? ?. inversion_mstep.
+      remember (EF_Alloc (length m) v) as eff.
+      induction_step; inversion Heqeff; subst; WBA.destruct_wba;
+      inversion_not_access; eauto using access, not_access_load. 
+      - intros ?. inversion_access; eauto.
+        rewrite (get_add_eq TM_Nil) in *.
+        eapply inaccessible_address_add_2; eauto. intros F.
+        specialize (Hwba (length m) F). lia.
+      - eapply not_access_asg; eauto. eapply inaccessible_address_add_2; eauto.
+        intros F. match goal with Hwba : well_behaved_access m ?t |- _ =>
+          specialize (Hwba (length m) F); lia
+        end.
+      - eapply not_access_asg; eauto; eapply inaccessible_address_add_2; eauto.
+        intros F. match goal with Hwba : well_behaved_access m ?t |- _ =>
+          specialize (Hwba (length m) F); lia
+        end.
+      - eapply not_access_seq; eauto; eapply inaccessible_address_add_2; eauto.
+        intros F. match goal with Hwba : well_behaved_access m ?t |- _ =>
+          specialize (Hwba (length m) F); lia
+        end.
     Qed.
   End Alloc.
 
@@ -362,7 +694,6 @@ Module MStep.
       try inversion_access; eauto using access.
     Qed.
 
-    (* unused *)
     Lemma preserves_access : forall m m' t t' ad ad' v,
       ad <> ad' ->
       access m t ad ->
@@ -392,8 +723,8 @@ Module MStep.
       m / t ==[EF_Load ad v]==> m' / t' ->
       access m t ad.
     Proof.
-      intros * Hmstep. inversion Hmstep; subst.
-      eauto using Step.load_ad_access.
+      intros. inversion_mstep. remember (EF_Load ad (getTM m' ad)) as eff.
+      induction_step; inversion Heqeff; subst; eauto using access.
     Qed.
   End Load.
 
@@ -402,7 +733,33 @@ Module MStep.
       m / t ==[EF_Store ad v]==> m' / t' ->
       access m t ad.
     Proof.
-      intros * ?. inversion_mstep. eauto using Step.Store.address_access.
+      intros * ?. inversion_mstep. remember (EF_Store ad v) as eff.
+      induction_step; inversion Heqeff; subst; eauto using access.
+    Qed.
+
+    Lemma inherits_access : forall m m' t t' ad ad' v,
+      access m' t' ad ->
+      m / t ==[EF_Store ad' v]==> m' / t' ->
+      access m t ad.
+    Proof.
+      intros. inversion_mstep. remember (EF_Store ad' v) as eff.
+      induction_step; inversion Heqeff; subst;
+      try inversion_access; eauto using access;
+      destruct (access_dec m v ad);
+      eauto using access, Step.Store.value_access, Mem.Set_.preserves_access.
+    Qed.
+
+    Lemma preserves_not_access : forall m m' t t' ad ad' v,
+      ~ access m t ad ->
+      m / t ==[EF_Store ad' v]==> m' / t' ->
+      ~ access m' t' ad.
+    Proof.
+      intros * Hnacc ?. inversion_mstep.
+      remember (EF_Store ad' v) as eff.
+      induction_step; inversion Heqeff; subst;
+      inversion_not_access;
+      eauto using not_access_load, not_access_asg, not_access_seq,
+                  Mem.Set_.preserves_not_access, Step.Store.value_not_access.
     Qed.
   End Store.
 End MStep.
